feat: directions now mean a thing, and large inductives exist

Reflection/MutualInductive.lean
@@ -8,7 +8,7 @@ import Reflection.Util.EqHelpers
 -/
 
 set_option pp.proofs true
-set_option pp.universes true
+-- set_option pp.universes true
 set_option linter.unusedVariables false
 
 /--Direction of a parameter, describes whether it
@@ -20,63 +20,80 @@ inductive Dir where
   | geq
   | eq
 
+instance : EmptyCollection Dir := ⟨.none⟩
+notation "≤ₐ" => Dir.leq
+notation "≥ₐ" => Dir.geq
+notation "=ₐ" => Dir.eq
+
+def Dir.max : Dir → Dir → Dir
+  | none, d | d, none => d
+  | leq, geq | geq, leq | eq, _ | _, eq => eq
+  | leq, leq => leq
+  | geq, geq => geq
+
+def Dir.LE : Dir → Dir → Prop
+  | .none , _
+  | _,=ₐ => True
+  | ≤ₐ,≤ₐ | ≥ₐ, ≥ₐ => True
+  | _,_ => False
+
+instance : LE Dir := ⟨Dir.LE⟩
+
 -- # Syntax
 
 /-- Example for `Nat` is `@U []`, for `List` is `@U [leq]`. -/
 inductive Tyₛ (l : List Dir): Type u
 | U : Tyₛ l
 -- No need to work on indexed inductives just yet, let's focus on polymorphic types first
--- | SArr : (T : Type u) -> Tyₛ -> Tyₛ
+-- | SArr : (T : Type u) → Tyₛ → Tyₛ
 open Tyₛ
 
 inductive Conₛ (l : List Dir)
 | nil : Conₛ l
-| cons : Tyₛ l -> Conₛ l -> Conₛ l
+| cons : Tyₛ l → Conₛ l → Conₛ l
 notation "[]" => Conₛ.nil
 infixr:67 " :: " => Conₛ.cons
 
 /-- De-brujin variable referring to an entry in the context.
 A context is for example `["Even", "Odd"]`, then `.vz` refers to `"Even"`.
 These are nameless, the quotations are only to ease explanation. -/
-inductive Varₛ : Conₛ l -> Tyₛ l -> Type u
-| vz :               Varₛ (Aₛ :: Γₛ) Aₛ
-| vs : Varₛ Γₛ Aₛ -> Varₛ (Bₛ :: Γₛ) Aₛ
+inductive Varₛ : Conₛ l → Tyₛ l → Type u
+| vz : Varₛ (Aₛ :: Γₛ) Aₛ
+| vs : Varₛ Γₛ Aₛ → Varₛ (Bₛ :: Γₛ) Aₛ
 open Varₛ
 
-inductive Varₚ : List Dir → Type (u+1)
-| vz : Varₚ [A]
-| vs : Varₚ l -> Varₚ (Bₛ :: l)
+inductive Varₚ (d : Dir): List Dir → Type (u+1)
+| vz : d ≤ d' → Varₚ d [d']
+| vs : Varₚ d l → Varₚ d (Bₛ :: l)
 
 /-- `t : Tmₛ Γ A` corresponds to `Γ ⊢ t : A`.
 Original Agda: https://bitbucket.org/javra/inductive-families/src/717f404c220e17d0ac5917306fd74dd0c4883cde/agda/IF.agda#lines-25:27 -/
-inductive Tmₛ.{u} : Conₛ.{u} l -> Tyₛ.{u} l -> Type (u+1)
+inductive Tmₛ.{u}: Conₛ.{u} l → Tyₛ.{u} l → Dir → Type (u+1)
 /-- A variable is a term.
 ```-
 (a : A) ∈ Γ
 -----------varInd
 Γ ⊢ₛ a : A
 ``` -/
-| varInd : Varₛ Γ A -> Tmₛ Γ A
+| varInd : Varₛ Γ A → Tmₛ Γ A d
 /-- Function application.
 ```-
 A ∈ l
 -----------varParam
 Γ ⊢ₛ A : Type
 ``` -/
-| varParam : Varₚ l → Tmₛ Γ (@U l)
-infixl:50 " @ " => Tmₛ.app
+| varParam : Varₚ d l → Tmₛ Γ (@U l) d
+| arr : (T : Type u) → Tmₛ Γ A d → Tmₛ Γ A d
+| param : Varₚ (d.max ≥ₐ) l → Tmₛ Γ A (d.max ≤ₐ) → Tmₛ Γ (@U l) d
 
--- -- ! This fails:
--- gen_injective_theorems% Tmₛ
+/-- Constructor types `... → Self ...`.
 
-/-- Constructor types `... -> Self ...`.
-
-Example `"(n : Nat) -> A -> Vec n -> Vec (n + 1)"`:
+Example `"(n : Nat) → A → Vec n → Vec (n + 1)"`:
 ```
 def V_cons (A : Type) : Tyₚ Vₛ :=
-  PPi Nat fun n => -- (n : Nat) ->
-    PPi A fun _ => -- A ->
-      PFunc ((Tmₛ.var vz) @ n) <| -- Vec n ->
+  PPi Nat fun n => -- (n : Nat) →
+    PPi A fun _ => -- A →
+      PFunc ((Tmₛ.var vz) @ n) <| -- Vec n →
         El ((Tmₛ.var vz) @ (n + 1)) -- Vec (n + 1)
 ```
 
@@ -84,14 +101,11 @@ The only way to create a `Tyₚ` is by ending it with a `El`, which must be a te
 The only way to create a term like that is by using `Tmₛ.app` and `Tmₛ.var`.
 For example the variables are `Even` and `Odd`, i.e. the other types in the mutual block being defined,
 then `Even @ 123` is a term in universe `U`. -/
-inductive Tyₚ : Conₛ l -> Type (u+1)
-| El : Tmₛ.{u} Γₛ U -> Tyₚ Γₛ
+inductive Tyₚ : Conₛ l →  Type (u+1)
+| El : Varₛ.{u} Γₛ U → Tyₚ Γₛ
 -- No need to work with dependent types just yet.
-| PArr   : (T : Type u) -> Tyₚ Γₛ -> Tyₚ Γₛ
-/-- Allows us to introduce nested binders `(x : Self ...) -> ...`.
-  `PFunc` is non-dependent, because it makes no sense to have `(self : Self ...) -> Self self`.
-  (...but once you have ind-ind or ind-rec, it might be sensible?) -/
-| PFunc : Tmₛ Γₛ U   -> Tyₚ Γₛ  -> Tyₚ Γₛ
+| PArr : (T : Type u) → Tyₚ Γₛ → Tyₚ Γₛ
+| PFunc : Tmₛ Γₛ U ∅ → Tyₚ Γₛ → Tyₚ Γₛ
 open Tyₚ
 
 /-- List of constructor descriptions.
@@ -106,27 +120,38 @@ V_nil :: V_cons A :: []
 ``` -/
 inductive Conₚ (Γ : Conₛ l): Type (u+1)
 | nil : Conₚ Γ
-| cons : Tyₚ Γ -> Conₚ Γ -> Conₚ Γ
+| cons : Tyₚ Γ → Conₚ Γ → Conₚ Γ
 notation "[]" => Conₚ.nil
 infixr:67 " :: " => Conₚ.cons
 
 section Examples
   /-- Corresponds to `Nat : U`. -/
   def Nₛ : Conₛ .nil := U :: []
-  /-- Corresponds to the two constructors `Nat.zero : Nat` and `Nat.succ : Nat -> Nat`. -/
-  def N  : Conₚ Nₛ := El (.varInd .vz) :: PFunc (.varInd .vz) (El (.varInd .vz)) :: []
+  /-- Corresponds to the two constructors `Nat.zero : Nat` and `Nat.succ : Nat → Nat`. -/
+  def N  : Conₚ Nₛ := El .vz :: PFunc (.varInd .vz) (El .vz) :: []
 
   -- List : Type → U
-  def Vₛ : Conₛ [.none] := U :: []
+  def Vₛ : Conₛ [≤ₐ] := U :: []
 
   -- List : Type → U ⊢ₛ  List A : U
-  def V_nil : Tyₚ Vₛ := El (.varInd .vz) -- List A
+  def V_nil : Tyₚ Vₛ := El .vz -- List A
 
   -- List : Type → U ⊢ₛ  A → List A → List A
   def V_cons : Tyₚ Vₛ :=
-    PFunc (Tmₛ.varParam .vz) <| -- A →
-      PFunc (Tmₛ.varInd vz) <| -- List A ->
-        El (Tmₛ.varInd vz) -- List A
+    PFunc (Tmₛ.varParam (.vz ⟨⟩)) <| -- A →
+      PFunc (Tmₛ.varInd vz) <| -- List A →
+        El vz -- List A
+
+/--Example of a constructor that cannot be valid.
+   `V_invalid : A → (A → List A) → List A`
+   `A` appears in a contravariant position despite being marked as covariant.
+   As such, the `sorry` cannot be proven.
+-/
+  def V_invalid : Tyₚ Vₛ  :=
+    PFunc (Tmₛ.varParam (.vz ⟨⟩)) <| -- A →
+                      --vvvvvv this is not provable, it's just false really
+      PFunc (.param (.vz sorry) (Tmₛ.varInd vz)) <| -- (A → List A) →
+        El vz -- List A
 
   def V : Conₚ Vₛ := V_nil :: V_cons :: []
 end Examples
@@ -147,16 +172,22 @@ def List.Telescope.bind (l : List Dir) (x : List.Telescope l A) (f : A → List.
     | .nil => f x
     | .cons hd tl => fun h : Type _ => List.Telescope.bind tl (x h) (fun y => f y h)
 
+def List.Telescope.run (l : List Dir) (params : List (Type u))
+(h : l.length = params.length) (tel : l.Telescope A): A :=
+match l,params with
+  | .nil,.nil => tel
+  | .cons _ tl₁,.cons T tl₂ => List.Telescope.run tl₁ tl₂ (by simp_all) (tel T)
+
 instance : Monad (List.Telescope l) where
   pure := List.Telescope.pure l
   bind := List.Telescope.bind l
 
-/-- Interprets a sort type, for example `SPi Nat (fun n => U)` becomes `Nat -> Type`. -/
-def TyₛA : Tyₛ.{u} l -> Type (u+1) := fun _ => (Type u)
--- | SPi T A => (t : T) -> TyₛA (A t)
+/-- Interprets a sort type, for example `SPi Nat (fun n => U)` becomes `Nat → Type`. -/
+def TyₛA : Tyₛ.{u} l → Type (u+1) := fun _ => (Type u)
+-- | SPi T A => (t : T) → TyₛA (A t)
 
-/-- Interprets a context of type formers.  The `Vec` example becomes `(Nat -> Type) × Unit`. -/
-def ConₛA' : Conₛ l -> Type (u+1)
+/-- Interprets a context of type formers.  The `Vec` example becomes `(Nat → Type) × Unit`. -/
+def ConₛA' : Conₛ l → Type (u+1)
   | .nil => PUnit
   | .cons A Γ => Prod (TyₛA A) (ConₛA' Γ)
 termination_by structural Γₛ => Γₛ
@@ -170,7 +201,7 @@ example : ConₛA Vₛ = (Type → (Type × PUnit.{2})) := by rfl
   we find the interpretation that we care about.
   Note that `γₛ` is a "list" with `List.cons` replaced with `Prod.mk`.
 
-  For example if `Γₛ` is `["(n:Nat) -> U"]`, and if `γₛ` is `⟨Vec, ()⟩`,
+  For example if `Γₛ` is `["(n:Nat) → U"]`, and if `γₛ` is `⟨Vec, ()⟩`,
   then `VarₛA vz γₛ` will reduce to `Vec`.
 
   This function returns an actual (unquoted) Lean type, e.g. `Vec`.
@@ -182,17 +213,17 @@ def VarₛA {Γₛ : Conₛ l} (v : Varₛ Γₛ Aₛ) (c : ConₛA Γₛ): l.Te
     |  vs v, ⟨_, γₛ⟩ => VarₛA v (pure γₛ)
 
 
-def VarₚA : {l : List Dir} → Varₚ l -> l.Telescope (Type u)
+def VarₚA : {l : List Dir} → Varₚ l → l.Telescope (Type u)
 |  [d], .vz  => fun A => A
 | _   :: l, .vs v => fun _ => VarₚA v
 
 /-- A `Vec` example in pseudocode, where quotation marks refer to object language:
 ```
-@TmₛA ["Nat -> Type"] "Type" "Vec 123" ⟨Vec, ()⟩
+@TmₛA ["Nat → Type"] "Type" "Vec 123" ⟨Vec, ()⟩
 ```
 reduces to:
 ```
-(@TmₛA ["Nat -> Type"] "Type" "Vec" ⟨Vec, ()⟩) 123
+(@TmₛA ["Nat → Type"] "Type" "Vec" ⟨Vec, ()⟩) 123
 ```
 reduces to:
 ```
@@ -228,7 +259,7 @@ TyₚA (V_cons A) ⟨Vec, ⟨⟩⟩
 ```
 reduces to the type of `Vec.cons` as you would expect:
 ```
-(n : Nat) -> A -> Vec n -> Vec (n + 1)
+(n : Nat) → A → Vec n → Vec (n + 1)
 ``` -/
 def TyₚA.{u} {Γₛ : Conₛ.{u} l} (t : Tyₚ.{u} Γₛ) (γₛ : ConₛA.{u} Γₛ): l.Telescope (Type u) :=
 match t with
@@ -262,10 +293,10 @@ ConₚA (V_nil :: V_cons A :: []) ⟨Vec, ⟨⟩⟩
 reduces to the Lean type
 ```
   (Vec 0) -- `Vec.nil`
-× ((n : Nat) -> A -> Vec n -> Vec (n + 1)) -- `Vec.cons`
+× ((n : Nat) → A → Vec n → Vec (n + 1)) -- `Vec.cons`
 × Unit
 ``` -/
-def ConₚA.{u} {Γₛ : Conₛ.{u} l} : Conₚ.{u} Γₛ -> ConₛA.{u} Γₛ -> l.Telescope (Type u)
+def ConₚA.{u} {Γₛ : Conₛ.{u} l} : Conₚ.{u} Γₛ → ConₛA.{u} Γₛ → l.Telescope (Type u)
 | .nil, _ => pure PUnit.{u+1}
 | .cons A Γ, γₛ => do
   let t₁ ← TyₚA.{u} A γₛ
@@ -274,17 +305,17 @@ def ConₚA.{u} {Γₛ : Conₛ.{u} l} : Conₚ.{u} Γₛ -> ConₛA.{u} Γₛ -
 
 example {List : Type → Type} {A : type}
   : ConₚA V (fun A => ⟨List A, ⟨⟩⟩)
-  = fun A => (List A × (A -> List A -> List A) × Unit)
+  = fun A => (List A × (A → List A → List A) × Unit)
   := rfl
 
 -- ## Displayed Algebras
 
 /-- Compute motive type.
 
-Example: `TyₛD (SPi Nat (fun _ => U)) Vec` reduces to `(n : Nat) -> Vec n -> Type`. -/
-def TyₛD.{u} (Aₛ : Tyₛ.{u} l) : TyₛA.{u} Aₛ -> Type u :=
-  fun T => T -> Sort u
--- | SPi T Aₛ, f => (t : T) -> TyₛD (Aₛ t) (f t)
+Example: `TyₛD (SPi Nat (fun _ => U)) Vec` reduces to `(n : Nat) → Vec n → Type`. -/
+def TyₛD.{u} (Aₛ : Tyₛ.{u} l) : TyₛA.{u} Aₛ → Type u :=
+  fun T => T → Sort u
+-- | SPi T Aₛ, f => (t : T) → TyₛD (Aₛ t) (f t)
 
 /-- Compute motive type for each mutually defined inductive type.
 
@@ -294,7 +325,7 @@ ConₛD Vₛ ⟨Vec, ⟨⟩⟩
 ```
 reduces to just one motive type:
 ```
-((t : Nat) → Vec t -> Type) × Unit
+((t : Nat) → Vec t → Type) × Unit
 ``` -/
 def ConₛD.{u} (Γₛ : Conₛ.{u} l) (c : ConₛA.{u} Γₛ): l.Telescope (Type u) :=
 match Γₛ with
@@ -303,9 +334,11 @@ match Γₛ with
   let ⟨a,γ⟩ ← c
   return (TyₛD A a) × (← ConₛD Γ (pure γ))
 
-example : ConₛD Vₛ (fun A => ⟨List A, ⟨⟩⟩) = fun A : Type => ((List A -> Prop) × PUnit.{1}) := rfl
+example : ConₛD Vₛ (fun A => ⟨List A, ⟨⟩⟩) = fun A : Type => ((List A → Prop) × PUnit.{1}) := rfl
 
-def VarₛD {Γₛ : Conₛ.{u} l}: (v : Varₛ Γₛ Aₛ) -> ConₛD Γₛ γₛ -> TyₛD Aₛ (VarₛA v γₛ)
+def VarₛD {Γₛ : Conₛ.{u} l} (params : List (Type u))
+  (h : l.length = params.length) (v : Varₛ Γₛ Aₛ) (γₛ : List.Telescope.run l params h (ConₛD Γₛ γₛ ))
+: TyₛD Aₛ (VarₛA v (pure γₛ))
 | .vz  , ⟨a, _⟩ => a
 | .vs v, ⟨a, γD⟩ => VarₛD v γD
 
@@ -320,7 +353,7 @@ for this is, again with `VarₛD` inlined:
 ``` -/
 -- ! TmₛD needs casts because reduction behaviour of TmₛA is broken.
 -- And for some reason TmₚD works just fine? What...
-def TmₛD : {Γₛ : Conₛ} -> {Aₛ : Tyₛ} -> {γₛ : ConₛA Γₛ} -> (t : Tmₛ  Γₛ Aₛ) -> ConₛD Γₛ γₛ -> TyₛD Aₛ (TmₛA t γₛ)
+def TmₛD : {Γₛ : Conₛ} → {Aₛ : Tyₛ} → {γₛ : ConₛA Γₛ} → (t : Tmₛ  Γₛ Aₛ) → ConₛD Γₛ γₛ → TyₛD Aₛ (TmₛA t γₛ)
 |  _, _, _γₛ, .var v                    , γₛD => TmₛA_var.symm ▸ VarₛD v γₛD
 -- | Γₛ, _, γₛ, .app (T := T) (A := A) t u, γₛD => TmₛA_app.symm ▸ TmₛD t γₛD u
 
@@ -335,25 +368,25 @@ theorem TmₛD_var : TmₛD (Tmₛ.var v) γₛD = TmₛA_var.symm ▸ VarₛD v
 Example:
 ```
 @TyₚD Vₛ ⟨Vec A, ⟨⟩⟩ V_cons ⟨P, ⟨⟩⟩ Vec.cons
-  = ((n : Nat) -> (a : A) -> (v : Vec A n) -> P n v -> P (n + 1) (Vec.cons n a v))
+  = ((n : Nat) → (a : A) → (v : Vec A n) → P n v → P (n + 1) (Vec.cons n a v))
 ``` -/
 -- Note: The `Self` here can be a little misleading, as it may be a nested type with different indices.
-def TyₚD.{u, v} : (A : Tyₚ.{u} Γₛ) -> ConₛD.{u} Γₛ γₛ -> TyₚA.{u, v} A γₛ -> Type (max u v)
+def TyₚD.{u, v} : (A : Tyₚ.{u} Γₛ) → ConₛD.{u} Γₛ γₛ → TyₚA.{u, v} A γₛ → Type (max u v)
 | El         Self, γD, self => TmₛD Self γD self
-| PArr   T    Rest, γD, f   => (t : T) -> TyₚD Rest γD (f t)
-| PFunc Self Rest, γD, f    => ⦃self : TmₛA Self γₛ⦄ -> TmₛD Self γD self -> TyₚD Rest γD (f self)
+| PArr   T    Rest, γD, f   => (t : T) → TyₚD Rest γD (f t)
+| PFunc Self Rest, γD, f    => ⦃self : TmₛA Self γₛ⦄ → TmₛD Self γD self → TyₚD Rest γD (f self)
 
-inductive Vec (A : Type) : Nat -> Type
+inductive Vec (A : Type) : Nat → Type
 | nil : Vec A 0
-| cons : (n : Nat) -> A -> Vec A n -> Vec A (n + 1)
+| cons : (n : Nat) → A → Vec A n → Vec A (n + 1)
 
-example {A : Type} {P : List A -> Type}
+example {A : Type} {P : List A → Type}
   : @TyₚD Vₛ ⟨List A, ⟨⟩⟩ V_nil ⟨P, ⟨⟩⟩ List.nil
   = P List.nil
   := rfl
-example {A : Type} {P : List A -> Type}
+example {A : Type} {P : List A → Type}
   : @TyₚD Vₛ ⟨List A, ⟨⟩⟩ V_cons ⟨P, ⟨⟩⟩ List.cons
-  = ((a : A) -> (v : List A) -> P v -> P (List.cons a v))
+  = ((a : A) → (v : List A) → P v → P (List.cons a v))
   := rfl
 
 /-- Example:
@@ -363,18 +396,18 @@ example {A : Type} {P : List A -> Type}
 reduces to
 ```
   P 0 Vec.nil
-× ((n : Nat) -> (a : A) -> (v : Vec A n) -> P n v -> P (n + 1) (Vec.cons n a v))
+× ((n : Nat) → (a : A) → (v : Vec A n) → P n v → P (n + 1) (Vec.cons n a v))
 × PUnit
 ``` -/
-def ConₚD.{u, v} : (Γ : Conₚ.{u} Γₛ) -> ConₛD.{u, v} Γₛ γₛ -> ConₚA.{u, v} Γ γₛ -> Type (max u v)
+def ConₚD.{u, v} : (Γ : Conₚ.{u} Γₛ) → ConₛD.{u, v} Γₛ γₛ → ConₚA.{u, v} Γ γₛ → Type (max u v)
 | .nil, _, _ => PUnit
 | .cons A Γ, γD, ⟨a, γ⟩ => TyₚD A γD a × ConₚD Γ γD γ
 
-example {P : List A -> Type}
+example {P : List A → Type}
   : @ConₚD Vₛ ⟨List A, ⟨⟩⟩ (V_nil :: V_cons :: []) ⟨P, ⟨⟩⟩ ⟨List.nil, List.cons, ⟨⟩⟩
   = (
         (P List.nil)
-      × ((a : A) -> (v : List A) -> P v -> P (List.cons a v))
+      × ((a : A) → (v : List A) → P v → P (List.cons a v))
       × Unit
     )
   := rfl
@@ -389,13 +422,13 @@ TyₛS (SPi Nat (fun _ => U)) (Vec A) (fun _ _ => R)
 ```
 reduces to
 ```
-(n : Nat) -> (v : Vec A n) -> R
+(n : Nat) → (v : Vec A n) → R
 ``` -/
-def TyₛS.{u, v} : (Aₛ : Tyₛ.{u}) -> (αₛ : TyₛA.{u, v} Aₛ) -> TyₛD.{u, v} Aₛ αₛ -> Type (max u v)
-| U       , T , TD  => (t : T) -> TD t
--- | SPi T Aₛ, fₛ, fₛd => (t : T) -> TyₛS (Aₛ t) (fₛ t) (fₛd t)
+def TyₛS.{u, v} : (Aₛ : Tyₛ.{u}) → (αₛ : TyₛA.{u, v} Aₛ) → TyₛD.{u, v} Aₛ αₛ → Type (max u v)
+| U       , T , TD  => (t : T) → TD t
+-- | SPi T Aₛ, fₛ, fₛd => (t : T) → TyₛS (Aₛ t) (fₛ t) (fₛd t)
 
--- example {A R} : TyₛS (SPi Nat (fun _ => U)) (Vec A) (fun _ _ => R) = ((n : Nat) -> (v : Vec A n) -> R) := rfl
+-- example {A R} : TyₛS (SPi Nat (fun _ => U)) (Vec A) (fun _ _ => R) = ((n : Nat) → (v : Vec A n) → R) := rfl
 
 /-- Example:
 ```
@@ -403,16 +436,16 @@ ConₛS Vₛ ⟨Vec A, ⟨⟩⟩ ⟨fun _ _ => R, ⟨⟩⟩
 ```
 reduces to
 ```
-  ((n : Nat) -> (v : Vec A n) -> R)
+  ((n : Nat) → (v : Vec A n) → R)
 × PUnit
 ``` -/
-def ConₛS.{u, v} : (Γₛ : Conₛ.{u}) -> (γₛ : ConₛA.{u, v} Γₛ) -> ConₛD.{u, v} Γₛ γₛ -> Type (max u v)
+def ConₛS.{u, v} : (Γₛ : Conₛ.{u}) → (γₛ : ConₛA.{u, v} Γₛ) → ConₛD.{u, v} Γₛ γₛ → Type (max u v)
 | .nil, ⟨⟩, ⟨⟩ => PUnit
 | .cons Aₛ Γₛ, ⟨αₛ, γₛ⟩, ⟨αₛd, γₛd⟩ => TyₛS Aₛ αₛ αₛd × ConₛS Γₛ γₛ γₛd
 
--- example {A R} : ConₛS Vₛ ⟨Vec A, ⟨⟩⟩ ⟨fun _ _ => R, ⟨⟩⟩ = (((n : Nat) -> (v : Vec A n) -> R) × Unit) := rfl
+-- example {A R} : ConₛS Vₛ ⟨Vec A, ⟨⟩⟩ ⟨fun _ _ => R, ⟨⟩⟩ = (((n : Nat) → (v : Vec A n) → R) × Unit) := rfl
 
-def VarₛS : (x : Varₛ Γₛ Aₛ) -> ConₛS Γₛ γₛ γD -> TyₛS Aₛ (VarₛA x γₛ) (VarₛD x γD)
+def VarₛS : (x : Varₛ Γₛ Aₛ) → ConₛS Γₛ γₛ γD → TyₛS Aₛ (VarₛA x γₛ) (VarₛD x γD)
 | .vz  , ⟨αₛS, γₛS⟩ => αₛS
 | .vs v, ⟨ _, γₛS⟩ => VarₛS v γₛS
 
@@ -421,27 +454,27 @@ theorem TyₛS_helper {Aₛ : Tyₛ} {a b : TyₛA Aₛ} (hA : a = b) (d : Tyₛ
   : TyₛS Aₛ a d = TyₛS Aₛ b (hA ▸ d)
   := by subst hA; rfl
 
-def TmₛS : {Γₛ : Conₛ} -> {Aₛ : Tyₛ} -> {γₛ : ConₛA Γₛ} -> {γₛD : ConₛD Γₛ γₛ} ->
-  (t : Tmₛ Γₛ Aₛ) -> ConₛS Γₛ γₛ γₛD -> TyₛS Aₛ (TmₛA t γₛ) (TmₛD t γₛD)
+def TmₛS : {Γₛ : Conₛ} → {Aₛ : Tyₛ} → {γₛ : ConₛA Γₛ} → {γₛD : ConₛD Γₛ γₛ} →
+  (t : Tmₛ Γₛ Aₛ) → ConₛS Γₛ γₛ γₛD → TyₛS Aₛ (TmₛA t γₛ) (TmₛD t γₛD)
 | Γₛ, Aₛ, γₛ, γₛD, .var v, γₛS => by
   have hA : TmₛA (Tmₛ.var v) γₛ = VarₛA v γₛ := TmₛA_var
   rw [TyₛS_helper hA (TmₛD (Tmₛ.var v) γₛD), TmₛD_var, eq_symm_cancel hA]
   exact VarₛS v γₛS
 
-def TyₚS : (A : Tyₚ Γₛ) -> ConₛS Γₛ γₛ γₛD -> (α : TyₚA A γₛ) -> TyₚD A γₛD α -> Prop
+def TyₚS : (A : Tyₚ Γₛ) → ConₛS Γₛ γₛ γₛD → (α : TyₚA A γₛ) → TyₚD A γₛD α → Prop
 | El         Self, γₛS, α, αD =>                          TmₛS Self γₛS α = αD -- note the equality here!
-| PArr   T    Rest, γₛS, f, fD => (t    : T)         -> TyₚS Rest γₛS (f t)    (fD t)
-| PFunc Self Rest, γₛS, f, fD => (self : TmₛA Self γₛ) ->
+| PArr   T    Rest, γₛS, f, fD => (t    : T)         → TyₚS Rest γₛS (f t)    (fD t)
+| PFunc Self Rest, γₛS, f, fD => (self : TmₛA Self γₛ) →
   -- fD : {self : TmₛA Self γₛ} → TmₛD Self γD self → TyₚD Rest γD (f self)
   TyₚS  Rest    γₛS (f self) (@fD self (TmₛS Self γₛS self))
 
-def ConₚS : (Γ : Conₚ Γₛ) -> ConₛS Γₛ γₛ γₛD -> (γ : ConₚA Γ γₛ) -> ConₚD Γ γₛD γ -> Prop
+def ConₚS : (Γ : Conₚ Γₛ) → ConₛS Γₛ γₛ γₛD → (γ : ConₚA Γ γₛ) → ConₚD Γ γₛD γ → Prop
 | .nil     ,   _,     ⟨⟩,       ⟨⟩ => True
 | .cons A Γ, γₛS, ⟨α, γ⟩, ⟨αD, γD⟩ => TyₚS A γₛS α αD ∧ ConₚS Γ γₛS γ γD
 
 -- example : @ConₚS Vₛ ⟨Vec A, ⟨⟩⟩ ⟨Q, ⟨⟩⟩ (V A) ⟨f, ⟨⟩⟩ ⟨Vec.nil, Vec.cons, ⟨⟩⟩ ⟨nilD, consD, ⟨⟩⟩
 --   = (f 0 Vec.nil = nilD
---     ∧ ((n : Nat) -> (a : A) -> (v : Vec A n) -> (f (n + 1) (Vec.cons n a v) = consD n a /- v -/ (f n v)))
+--     ∧ ((n : Nat) → (a : A) → (v : Vec A n) → (f (n + 1) (Vec.cons n a v) = consD n a /- v -/ (f n v)))
 --     ∧ True)
 --   := rfl
 
@@ -452,31 +485,31 @@ def ConₚS : (Γ : Conₚ Γₛ) -> ConₛS Γₛ γₛ γₛD -> (γ : ConₚA
 Note that `Subₛ` is essentially a list of the same length as the context `Δₛ`.
 This is because for every entry in the context Δₛ we will substitute it
 with a Γₛ-term saved in `Subₛ`, thus the resulting context will be Γₛ.  -/
-inductive Subₛ : (Γₛ : Conₛ) -> (Δₛ : Conₛ) -> Type (u+1)
+inductive Subₛ : (Γₛ : Conₛ) → (Δₛ : Conₛ) → Type (u+1)
 | nil : Subₛ Γₛ .nil
-| cons : Subₛ Γₛ Δₛ -> Tmₛ Γₛ Aₛ -> Subₛ Γₛ (Aₛ :: Δₛ)
+| cons : Subₛ Γₛ Δₛ → Tmₛ Γₛ Aₛ → Subₛ Γₛ (Aₛ :: Δₛ)
 
 /-- Substitutes a variable `v ∈ Δₛ` with a Γₛ-term. -/
-def SubₛVar : Varₛ Δₛ Aₛ -> Subₛ Γₛ Δₛ -> Tmₛ Γₛ Aₛ
+def SubₛVar : Varₛ Δₛ Aₛ → Subₛ Γₛ Δₛ → Tmₛ Γₛ Aₛ
 | .vz  , .cons _ t => t
 | .vs v, .cons σ _ => SubₛVar v σ
 
 /-- Applies the substitution to a term, resulting in a new term in the new context. -/
-def SubₛTm : {Aₛ : _} -> Tmₛ Δₛ Aₛ -> Subₛ Γₛ Δₛ -> Tmₛ Γₛ Aₛ
+def SubₛTm : {Aₛ : _} → Tmₛ Δₛ Aₛ → Subₛ Γₛ Δₛ → Tmₛ Γₛ Aₛ
 | _, .var v, σ => SubₛVar v σ
 -- | _, .app (A := _A) t u, σ => .app (SubₛTm t σ) u
 
-def SubₛTy : Tyₚ Δₛ -> Subₛ Γₛ Δₛ -> Tyₚ Γₛ
+def SubₛTy : Tyₚ Δₛ → Subₛ Γₛ Δₛ → Tyₚ Γₛ
 | El Self, σ => El (SubₛTm Self σ)
 | PArr T Rest, σ => PArr T (SubₛTy Rest σ)
 | PFunc Self Rest, σ => PFunc (SubₛTm Self σ) (SubₛTy Rest σ)
 
-def SubₛCon : Conₚ Δₛ -> Subₛ Γₛ Δₛ -> Conₚ Γₛ
+def SubₛCon : Conₚ Δₛ → Subₛ Γₛ Δₛ → Conₚ Γₛ
 | [], _ => []
 | A :: Γ, σ => SubₛTy A σ :: SubₛCon Γ σ
 
 /-- Increment all de brujin indices in this term by one. -/
-def vshift : {Aₛ : Tyₛ} -> Tmₛ Γₛ Aₛ -> Tmₛ (Bₛ :: Γₛ) Aₛ
+def vshift : {Aₛ : Tyₛ} → Tmₛ Γₛ Aₛ → Tmₛ (Bₛ :: Γₛ) Aₛ
 | _, .var v => .var (.vs v)
 -- | _, .app (A := _A) t u => .app (vshift t) u
 
@@ -484,12 +517,12 @@ def vshift : {Aₛ : Tyₛ} -> Tmₛ Γₛ Aₛ -> Tmₛ (Bₛ :: Γₛ) Aₛ
   Given a substitution `σ` which replaces all variables `Δₛ ⊢ v` with terms `Γₛ ⊢ t`,
   the weakened substitution will replace all variables `Δₛ ⊢ v` with terms `Γₛ, Aₛ ⊢ t`.
   The stored terms thus need to be shifted using `vshift`. -/
-def weaken.{u} : {Γₛ Δₛ : Conₛ.{u}} -> {Aₛ : Tyₛ.{u}} -> Subₛ.{u} Γₛ Δₛ -> Subₛ (Aₛ :: Γₛ) Δₛ
+def weaken.{u} : {Γₛ Δₛ : Conₛ.{u}} → {Aₛ : Tyₛ.{u}} → Subₛ.{u} Γₛ Δₛ → Subₛ (Aₛ :: Γₛ) Δₛ
 | Γₛ, .nil    , Aₛ, .nil => .nil
 | Γₛ, Bₛ :: Δₛ, Aₛ, .cons σ t => Subₛ.cons (weaken σ) (vshift t)
 
 /-- Identity substitution. Does nothing (replaces all variables by itself). -/
-def Subₛ.id : (Γₛ : Conₛ) -> Subₛ Γₛ Γₛ
+def Subₛ.id : (Γₛ : Conₛ) → Subₛ Γₛ Γₛ
 | .nil => .nil
 | .cons _ Γₛ => .cons (weaken (Subₛ.id Γₛ)) (.var .vz)
 
@@ -508,7 +541,7 @@ theorem aux : @Eq (Tmₛ (Bₛ :: Γₛ) Aₛ) (vshift (SubₛVar v (Subₛ.id �
     -- rw [ih] at h
     sorry
 
-theorem SubₛVar_id : (v : Varₛ Γₛ Aₛ) -> SubₛVar v (Subₛ.id Γₛ) = Tmₛ.var v := fun v => by
+theorem SubₛVar_id : (v : Varₛ Γₛ Aₛ) → SubₛVar v (Subₛ.id Γₛ) = Tmₛ.var v := fun v => by
   induction v with
   | vz => rw [Subₛ.id]; rfl
   | @vs Γₛ Aₛ Bₛ v ih =>
@@ -522,96 +555,96 @@ theorem SubₛVar_id : (v : Varₛ Γₛ Aₛ) -> SubₛVar v (Subₛ.id Γₛ) 
     rw [<- aux]
     exact ih
 
-theorem SubₛTm_id : (t : Tmₛ Γₛ Aₛ) -> SubₛTm t (Subₛ.id Γₛ) = t
+theorem SubₛTm_id : (t : Tmₛ Γₛ Aₛ) → SubₛTm t (Subₛ.id Γₛ) = t
 | .var v => SubₛVar_id v
 -- | .app (A := Aₛ) t u => sorry
 
-def SubₛA : Subₛ Γₛ Δₛ -> ConₛA Γₛ -> ConₛA Δₛ
+def SubₛA : Subₛ Γₛ Δₛ → ConₛA Γₛ → ConₛA Δₛ
 | .nil     ,  _ => ⟨⟩
 | .cons σ t, γₛ => ⟨TmₛA t γₛ, SubₛA σ γₛ⟩
 
-def SubₛD : (σ : Subₛ Γₛ Δₛ) -> ConₛD Γₛ γₛ -> ConₛD Δₛ (SubₛA σ γₛ)
+def SubₛD : (σ : Subₛ Γₛ Δₛ) → ConₛD Γₛ γₛ → ConₛD Δₛ (SubₛA σ γₛ)
 | .nil, γₛD => ⟨⟩
 | .cons σ t, γₛD => ⟨TmₛD t γₛD, SubₛD σ γₛD⟩
 
-def SubₛS : (σ : Subₛ Γₛ Δₛ) -> ConₛS Γₛ γₛ γₛD -> ConₛS Δₛ (SubₛA σ γₛ) (SubₛD σ γₛD)
+def SubₛS : (σ : Subₛ Γₛ Δₛ) → ConₛS Γₛ γₛ γₛD → ConₛS Δₛ (SubₛA σ γₛ) (SubₛD σ γₛD)
 | .nil, γₛD => ⟨⟩
 | .cons σ t, γₛD => ⟨TmₛS t γₛD, SubₛS σ γₛD⟩
 
 
 -- ## Now for Points...
 
-inductive Varₚ : Conₚ Γₛ -> Tyₚ Γₛ -> Type (u+1)
+inductive Varₚ : Conₚ Γₛ → Tyₚ Γₛ → Type (u+1)
 | vz :               Varₚ (Aₛ :: Γₛ) Aₛ
-| vs : Varₚ Γₛ Aₛ -> Varₚ (Bₛ :: Γₛ) Aₛ
+| vs : Varₚ Γₛ Aₛ → Varₚ (Bₛ :: Γₛ) Aₛ
 
 set_option genInjectivity false in
-inductive Tmₚ.{u} {Γₛ : Conₛ.{u}} : Conₚ.{u} Γₛ -> Tyₚ.{u} Γₛ -> Type (u+1)
-| var : Varₚ Γ A -> Tmₚ Γ A
-| app {T : Type u} {A : Tyₚ Γₛ} : Tmₚ Γ (PArr T A)   -> (t : T)      -> Tmₚ Γ A
-| appr             {A :      Tyₚ Γₛ} : Tmₚ Γ (PFunc a A) -> Tmₚ Γ (El a) -> Tmₚ Γ A
+inductive Tmₚ.{u} {Γₛ : Conₛ.{u}} : Conₚ.{u} Γₛ → Tyₚ.{u} Γₛ → Type (u+1)
+| var : Varₚ Γ A → Tmₚ Γ A
+| app {T : Type u} {A : Tyₚ Γₛ} : Tmₚ Γ (PArr T A)   → (t : T)      → Tmₚ Γ A
+| appr             {A :      Tyₚ Γₛ} : Tmₚ Γ (PFunc a A) → Tmₚ Γ (El a) → Tmₚ Γ A
 
 /-- Represents a substitution from Δₛ to Γₛ.
 Note that `Subₛ` is essentially a list of the same length as the context `Δₛ`.
 This is because for every entry in the context Δₛ we will substitute it
 with a Γₛ-term saved in `Subₛ`, thus the resulting context will be Γₛ.  -/
-inductive Subₚ : (Γ : Conₚ Γₛ) -> (Δ : Conₚ Δₛ) -> Type (u+1)
+inductive Subₚ : (Γ : Conₚ Γₛ) → (Δ : Conₚ Δₛ) → Type (u+1)
 | nil : Subₚ Γ .nil
-| cons : Subₚ Γ Δ -> Tmₚ Γ A -> Subₚ Γ (A :: Δ)
+| cons : Subₚ Γ Δ → Tmₚ Γ A → Subₚ Γ (A :: Δ)
 
 /-- Substitutes a variable `v ∈ Δₛ` with a Γₛ-term. -/
-def SubₚVar : Varₚ Δ A -> Subₚ Γ Δ -> Tmₚ Γ A
+def SubₚVar : Varₚ Δ A → Subₚ Γ Δ → Tmₚ Γ A
 | .vz  , .cons _ t => t
 | .vs v, .cons σ _ => SubₚVar v σ
 
 /-- Applies the substitution to a term, resulting in a new term in the new context. -/
-def SubₚTm : {A : Tyₚ Γₛ} -> Tmₚ Δ A -> Subₚ Γ Δ -> Tmₚ Γ A
+def SubₚTm : {A : Tyₚ Γₛ} → Tmₚ Δ A → Subₚ Γ Δ → Tmₚ Γ A
 | _, .var v, σ => SubₚVar v σ
 | _, .app (A := _A) t u, σ => .app (SubₚTm t σ) u
 | _, .appr (A := A) t u, σ => .appr (SubₚTm t σ) (SubₚTm u σ)
 
-def vsₚ : {A : Tyₚ Γₛ} -> Tmₚ Γ A -> Tmₚ (B :: Γ) A
+def vsₚ : {A : Tyₚ Γₛ} → Tmₚ Γ A → Tmₚ (B :: Γ) A
 | _, .var v => .var (.vs v)
 | _, .app (A := _A) t u => .app (vsₚ t) u
 | _, .appr (A := _A) t u => .appr (vsₚ t) (vsₚ u)
 
-def weakenₚ.{u} : {Γ Δ : Conₚ.{u} Γₛ} -> {A : Tyₚ.{u} Γₛ} -> Subₚ.{u} Γ Δ -> Subₚ (A :: Γ) Δ
+def weakenₚ.{u} : {Γ Δ : Conₚ.{u} Γₛ} → {A : Tyₚ.{u} Γₛ} → Subₚ.{u} Γ Δ → Subₚ (A :: Γ) Δ
 | _, .nil  , _, .nil => .nil
 | _, _ :: _, _, .cons σ t => Subₚ.cons (weakenₚ σ) (vsₚ t)
 
-def Subₚ.id : (Γ : Conₚ Γₛ) -> Subₚ Γ Γ
+def Subₚ.id : (Γ : Conₚ Γₛ) → Subₚ Γ Γ
 | .nil => .nil
 | .cons _ Γ => .cons (weakenₚ (Subₚ.id Γ)) (.var .vz)
 
 theorem SubₚTm_id (t : Tmₚ Γ A) : SubₚTm t (Subₚ.id Γ) = t := sorry
 
 
-def VarₚA : Varₚ Γ A -> ConₚA Γ γₛ -> TyₚA A γₛ
+def VarₚA : Varₚ Γ A → ConₚA Γ γₛ → TyₚA A γₛ
 | .vz  , ⟨a, _⟩ => a
 | .vs v, ⟨_, γ⟩ => VarₚA v γ
 
-def TmₚA.{u} : {A : Tyₚ Γₛ} -> Tmₚ.{u} Γ A -> ConₚA.{u} Γ γₛ -> TyₚA.{u} A γₛ
+def TmₚA.{u} : {A : Tyₚ Γₛ} → Tmₚ.{u} Γ A → ConₚA.{u} Γ γₛ → TyₚA.{u} A γₛ
 | _, .var v, γ => VarₚA v γ
 | _, .app (A := _A) t u, γ => (TmₚA t γ) u
 | _, .appr (A := _) t u, γ => (TmₚA t γ) (TmₚA u γ)
 
-def SubₚA : Subₚ Γ Δ -> ConₚA Γ γₛ -> ConₚA Δ γₛ
+def SubₚA : Subₚ Γ Δ → ConₚA Γ γₛ → ConₚA Δ γₛ
 | .nil     ,  _ => ⟨⟩
 | .cons σ t, γₛ => ⟨TmₚA t γₛ, SubₚA σ γₛ⟩
 
-def VarₚD : (x : Varₚ Γ A) -> ConₚD Γ γₛD γ -> TyₚD A γₛD (VarₚA x γ)
+def VarₚD : (x : Varₚ Γ A) → ConₚD Γ γₛD γ → TyₚD A γₛD (VarₚA x γ)
 | .vz  , ⟨aD, _⟩ => aD
 | .vs v, ⟨_, γD⟩ => VarₚD v γD
 
 -- This works but TmₛA_var doesn't work by rfl?
 theorem TmₚA_var : TmₚA (Tmₚ.var v) γₛ = VarₚA v γₛ := by rfl
 
-def TmₚD : (t : Tmₚ Γ A) -> ConₚD Γ γₛD γ -> TyₚD A γₛD (TmₚA t γ)
+def TmₚD : (t : Tmₚ Γ A) → ConₚD Γ γₛD γ → TyₚD A γₛD (TmₚA t γ)
 | .var v, γD => VarₚD v γD
 | .app (A := _A) t u, γD => TmₚD t γD u
 | .appr (A := A) t u, γD => TmₚD t γD (TmₚD u γD)
 
-def SubₚD : (σ : Subₚ Γ Δ) -> ConₚD Γ γₛD γ -> ConₚD Δ γₛD (SubₚA σ γ)
+def SubₚD : (σ : Subₚ Γ Δ) → ConₚD Γ γₛD γ → ConₚD Δ γₛD (SubₚA σ γ)
 | .nil, γD => ⟨⟩
 | .cons σ t, γD => ⟨TmₚD t γD, SubₚD σ γD⟩
 
@@ -635,12 +668,12 @@ constrTmₛ' (Ω := V String) (Ωₛ := Vₛ) (Aₛ := (SPi Nat (fun _ => U))) (
 ```
 reduces to
 ```
-fun (n : Nat) => Tmₚ (V String) (El ((.var .vz) @ n))    :   Nat -> Type
+fun (n : Nat) => Tmₚ (V String) (El ((.var .vz) @ n))    :   Nat → Type
 ```
-which is a stand-in for `Vec String : Nat -> Type`.
+which is a stand-in for `Vec String : Nat → Type`.
 We do not have an actual `Vec String`, so instead we use `constrTmₛ (V String)`
 -/
-def constrTmₛ' : {Aₛ : Tyₛ.{u}} -> Tmₛ.{u} Ωₛ Aₛ -> TyₛA.{u, u + 1} Aₛ -- baked-in ULift into TyₛA
+def constrTmₛ' : {Aₛ : Tyₛ.{u}} → Tmₛ.{u} Ωₛ Aₛ → TyₛA.{u, u + 1} Aₛ -- baked-in ULift into TyₛA
 | U      , t => Tmₚ Ω (El t)
 -- | SArr _ _, t => fun u => constrTmₛ' (.app t u)
 
@@ -653,7 +686,7 @@ def constrTmₛ' : {Aₛ : Tyₛ.{u}} -> Tmₛ.{u} Ωₛ Aₛ -> TyₛA.{u, u + 
 --   = fun (n : Nat) => Tmₚ (V String) (El ((.var .vz) @ n))
 --   := rfl
 
-def constrₛ' : Subₛ Ωₛ Γₛ -> ConₛA Γₛ
+def constrₛ' : Subₛ Ωₛ Γₛ → ConₛA Γₛ
 | .nil => ⟨⟩
 | .cons σ t => ⟨constrTmₛ' (Ω := Ω) t, constrₛ' σ⟩
 
@@ -692,15 +725,15 @@ example (t : Tmₛ Γₛ Aₛ) : (TmₛA t) ∘ (@constrₛ' Ωₛ Ω Γₛ) = (
 
 -- example
 --   : @TyₚA Vₛ (PPi Nat fun n => @El Vₛ ((.var vz) @ n)) (@constrₛ Vₛ (V String))
---   -- = ((n : Nat) -> (fun n => Tmₚ (V String) (El ((.var .vz) @ n))) n) -- intermediate step
---   = ((n : Nat) -> Tmₚ (V String) (El ((.var .vz) @ n)))
+--   -- = ((n : Nat) → (fun n => Tmₚ (V String) (El ((.var .vz) @ n))) n) -- intermediate step
+--   = ((n : Nat) → Tmₚ (V String) (El ((.var .vz) @ n)))
 --   := rfl
 -- example --       vvvvvvvvvvvvvvvvvv "Self"
 --   : @TyₚA Vₛ (El ((.var vz) @ 123)) (@constrₛ Vₛ (V String))
 --   = Tmₚ (V String) (El ((.var .vz) @ 123))
 --   := rfl
 
-def constrTmₚ' : {A : Tyₚ _} -> Tmₚ Ω A -> TyₚA A (constrₛ (Ω := Ω))
+def constrTmₚ' : {A : Tyₚ _} → Tmₚ Ω A → TyₚA A (constrₛ (Ω := Ω))
 | El Self, t => by
   -- this is actually `⊢ Tmₚ Ω (El Self)` but lean isn't smart enough
   rw [TyₚA]
@@ -718,7 +751,7 @@ def constrTmₚ' : {A : Tyₚ _} -> Tmₚ Ω A -> TyₚA A (constrₛ (Ω := Ω)
       exact u
     constrTmₚ' (.appr t u)
 
-def constrₚ' : Subₚ Ω Γ -> ConₚA Γ (constrₛ (Ω := Ω))
+def constrₚ' : Subₚ Ω Γ → ConₚA Γ (constrₛ (Ω := Ω))
 | .nil => ⟨⟩
 | .cons σ t => ⟨constrTmₚ' (Ω := Ω) t, constrₚ' σ⟩
 
@@ -732,7 +765,7 @@ theorem constrₚ_coherent (ttt : Tmₚ Γ A) (σ : Subₚ Ω Γ) : TmₚA ttt (
 
 variable (ωₛD : ConₛD Ωₛ constrₛ) (ωₛ : ConₚD Ω ωₛD constrₚ)
 
-def elimTmₛ' : {Aₛ : Tyₛ.{u}} -> (t : Tmₛ.{u} Ωₛ Aₛ) -> TyₛS.{u, u+1} Aₛ (TmₛA t (constrₛ (Ω:=Ω))) (TmₛD t ωₛD)
+def elimTmₛ' : {Aₛ : Tyₛ.{u}} → (t : Tmₛ.{u} Ωₛ Aₛ) → TyₛS.{u, u+1} Aₛ (TmₛA t (constrₛ (Ω:=Ω))) (TmₛD t ωₛD)
 | U, a =>
   -- a : Tmₛ Ωₛ U
   -- ⊢ TyₛS U (TmₛA a constrₛ) (TmₛD a ωₛD)
@@ -751,7 +784,7 @@ def elimTmₛ' : {Aₛ : Tyₛ.{u}} -> (t : Tmₛ.{u} Ωₛ Aₛ) -> TyₛS.{u, 
 --     simp only [eq_symm_cancel, eq_cast_trans] at res
 --     exact res
 
-def elimₛ' : (σ : Subₛ Ωₛ Γₛ) -> ConₛS Γₛ (SubₛA σ constrₛ) (SubₛD σ ωₛD)
+def elimₛ' : (σ : Subₛ Ωₛ Γₛ) → ConₛS Γₛ (SubₛA σ constrₛ) (SubₛD σ ωₛD)
 | .nil => ⟨⟩
 | .cons σ t => ⟨elimTmₛ' (Ω := Ω) ωₛD t, elimₛ' σ⟩
 
@@ -763,6 +796,6 @@ def elimₛ' : (σ : Subₛ Ωₛ Γₛ) -> ConₛS Γₛ (SubₛA σ constrₛ)
 namespace Example
   def List (A : Type) : Type 1                         := constrTmₛ' (Ω := V A) (.var .vz)
   def List.nil (A : Type) : List A                     := constrTmₚ' (Ω := V A) (.var .vz)
-  def List.cons (A : Type) : (x:A) -> List A -> List A := constrTmₚ' (Ω := V A) (.var (.vs .vz))
+  def List.cons (A : Type) : (x:A) → List A → List A := constrTmₚ' (Ω := V A) (.var (.vs .vz))
 
 end Example
